Start over, with codes and eval. Much simpler!

SimpleSets/Basic.lean
@@ -1,1 +1,377 @@
-def hello := "world"
+import Mathlib.Computability.Reduce
+
+
+#eval (Encodable.encode (Option.none : Option ℕ))
+#eval (Encodable.encode (Option.some 0 : Option ℕ))
+
+#print REPred
+
+-- A non-empty recursively enumerable set is the image of a primitive recursive function
+def PrimRecImage {β : Type} [Primcodable β] (B : Set β) :=
+  ∃ (f : ℕ → β), Primrec f ∧ ∀ b, b ∈ B ↔ ∃ a, f a ∈ B
+
+
+def boundedMin (f : ℕ → Bool) (n : ℕ) : ℕ :=
+  List.idxOf true <| List.map f (List.range n)
+
+@[simp]
+lemma boundedMin_zero (f : ℕ → Bool) :
+  boundedMin f 0 = 0 :=
+by
+  unfold boundedMin
+  simp [List.idxOf, List.range, List.range.loop]
+
+-- lemma idxOf_concat (f : ℕ → Bool) (n m : ℕ
+
+#print List.range.loop
+lemma range.aux (n : ℕ) (l : List ℕ) :
+  List.range.loop n l =
+  List.range n ++ l :=
+by
+  revert l
+  induction n <;> intro l
+  case zero =>
+    unfold List.range.loop
+    simp [List.map, List.range.loop]
+  case succ n ih =>
+    simp [List.range, List.range.loop]
+    rw [ih]
+    rw [ih]; simp [List.map, List.append_assoc]
+
+
+#print List.range'
+
+@[simp]
+lemma range_succ (n : ℕ) :
+  List.range (n+1) = List.range n ++ [n] :=
+by
+  unfold List.range
+  simp [List.range.loop]
+  apply range.aux
+
+
+lemma range_range' (n m : ℕ) :
+  List.range (n + m) = List.range n ++ List.range' n m :=
+by
+  revert n
+  induction m
+  case zero =>
+    simp [List.range, List.range.loop, List.range']
+  case succ m ih =>
+    intro n
+    simp [List.range', List.range.loop]
+    have h : (n + (m + 1)) = (n + 1) + m := by
+      omega
+    rw [h, ih]
+    simp
+
+#print List.findIdx.go
+
+lemma idxOf_cons₁ {α} [BEq α][ReflBEq α] (a : α) (l : List α) :
+  List.idxOf a (a :: l) = 0 :=
+by
+  simp [List.idxOf, List.findIdx, List.findIdx.go]
+
+lemma findIdx_aux {α} (f : α → Bool) (n m : ℕ) (l : List α) :
+  List.findIdx.go f l (n + m) = (List.findIdx.go f l n) + m :=
+  by
+  revert n m
+  induction l
+  case nil =>
+    unfold List.findIdx.go
+    simp [List.findIdx, List.findIdx.go]
+  case cons a l ih =>
+    simp [List.findIdx.go]
+    cases (f a)
+    case true =>
+      simp
+    case false =>
+      intro n m
+      simp [List.findIdx, List.findIdx.go]
+      have h : (n + m + 1) = (n + 1) + m := by
+        omega
+      rw [h, ih]
+
+lemma idxOf_cons₂ {α} [BEq α][LawfulBEq α] (a b : α) (l : List α) :
+  a ≠ b →
+  List.idxOf a (b :: l) = (List.idxOf a l) + 1 :=
+by
+  intro h
+  have h : b ≠ a := by symm; trivial
+  simp [List.idxOf, List.findIdx, List.findIdx.go]
+  rw [← beq_eq_false_iff_ne] at h
+  rw [h]
+  have h : 1 = (0 + 1) := by
+    omega
+  rw (occs := .pos [1]) [h]; rw [findIdx_aux]
+  simp
+
+
+lemma idxOf_concat₁ {α} [BEq α] [LawfulBEq α] (a : α) (l₁ l₂ : List α) :
+  a ∈ l₁ →
+  List.idxOf a (l₁ ++ l₂) = List.idxOf a l₁ :=
+by
+  revert l₂
+  induction l₁ <;> intro l₂
+  case nil =>
+    unfold List.idxOf
+    simp [List.append_nil]
+  case cons b l ih =>
+    simp
+    intro h; cases h
+    case inl h =>
+      rw [h, idxOf_cons₁]; simp [idxOf_cons₁]
+    case inr h =>
+      by_cases h: (a = b)
+      case pos => rw [h, idxOf_cons₁]; simp [idxOf_cons₁]
+      case neg =>
+      rw [idxOf_cons₂]; any_goals trivial
+      rw [idxOf_cons₂]; rw [ih]; trivial
+      trivial
+
+
+lemma idxOf_concat₂ {α} [BEq α] [LawfulBEq α] (a : α) (l₁ l₂ : List α) :
+  a ∉ l₁ →
+  List.idxOf a (l₁ ++ l₂) = l₁.length + List.idxOf a l₂ :=
+by
+  revert l₂
+  induction l₁
+  case nil =>
+    unfold List.idxOf
+    simp [List.append_nil]
+  case cons b l ih =>
+    simp; intros l₂ neq notin
+    rw [idxOf_cons₂]; swap; trivial
+    rw [ih]; omega; trivial
+
+
+
+#eval boundedMin (fun x => x == 5) 10
+#eval boundedMin (fun x => x == 12) 10
+
+theorem Primrec.boundedMinPrimrec (f : ℕ → Bool) :
+  Primrec f →
+  Primrec (boundedMin f) :=
+  by
+    intro primrec_f
+    unfold boundedMin
+    apply Primrec.comp
+    . apply Primrec₂.comp
+      . apply Primrec.list_idxOf
+      . apply Primrec.const
+      . apply Primrec.id
+    . apply Primrec.comp
+      . apply Primrec.list_map
+        . apply Primrec.id
+        . refine comp₂ primrec_f Primrec₂.right
+      . exact list_range
+
+def boundedMinOpt (f : ℕ → Bool) (n : ℕ) : Option ℕ :=
+  let idx := boundedMin f n
+  if idx < n then some idx else none
+
+lemma boundedMinRfind_mem (f : ℕ → Bool) (bound n : ℕ) :
+  n ∈ Nat.rfind f →
+  n < bound →
+  true ∈ List.map f (List.range bound) :=
+by
+  revert n
+  simp
+  induction bound
+  case zero =>
+    intro n h
+    simp [Nat.rfind, List.range]
+  case succ bound ih =>
+    intros n; intros; exists n
+
+
+lemma boundedMinRfind (f : ℕ → Bool) (bound n : ℕ) :
+  n ∈ Nat.rfind f →
+  n < bound →
+  boundedMin f bound = n :=
+by
+  intros mem; have mem' := mem; revert mem
+  simp
+  induction bound
+  case zero =>
+    intro _ _ _
+    omega
+  case succ bound ih =>
+    intro h1 h2 lt
+    simp [boundedMin]
+    have lt_case: n < bound ∨ n = bound := by
+      omega
+    cases lt_case
+    case inl lt =>
+      rw [idxOf_concat₁]
+      . apply ih <;> trivial
+      . apply boundedMinRfind_mem <;> trivial
+    case inr eq =>
+      rw [idxOf_concat₂]
+      . rw [← eq, h1]; simp
+      . simp; intros m ltm; apply h2; omega
+
+lemma boundedMinOptRfind (f : ℕ → Bool) (bound n : ℕ) :
+  n ∈ Nat.rfind f →
+  n < bound →
+  boundedMinOpt f bound = .some n :=
+by
+  intros mem lt
+  simp [boundedMinOpt]
+  have h1 := boundedMinRfind f bound n mem lt
+  constructor; omega; trivial
+
+theorem Primrec.boundedMinOptPrimrec (f : ℕ → Bool) :
+  Primrec f →
+  Primrec (boundedMinOpt f) :=
+  by
+    intro primrec_f
+    unfold boundedMinOpt
+    apply Primrec.ite
+    . apply Primrec₂.comp (f := λ x y ↦ decide <| x < y) (g := boundedMin f) (h := id)
+      . apply Primrec.nat_lt
+      . apply Primrec.boundedMinPrimrec; trivial
+      . apply Primrec.id
+    . apply Primrec.comp
+      . apply Primrec.option_some
+      . apply Primrec.boundedMinPrimrec; trivial
+    . apply Primrec.const
+
+#print Nat.Primrec
+#print Nat.Partrec
+
+-- Let's do this with codes: we associate a primitive recursive evaluator.
+
+#print Nat.Partrec.Code
+#print Nat.Partrec.Code.eval
+#check Nat.Partrec.Code.exists_code
+
+open Nat.Partrec (Code)
+
+def evalPrim : Code → ℕ → ℕ → Option ℕ
+| .zero, _, _ => some 0
+| .succ, _, n => some (n + 1)
+| .left, _, n => some n.unpair.1
+| .right, _, n => some n.unpair.2
+| .pair f g, bound, n =>
+  Nat.pair <$> evalPrim f bound n <*> evalPrim g bound n
+| .comp f g, bound, n =>
+  evalPrim g bound n >>= evalPrim f bound
+| .prec f g, bound, n =>
+  Nat.unpaired (fun a m =>
+    Nat.rec (evalPrim f bound a)
+    (fun y IH ↦ do
+      let i ← IH
+      evalPrim g bound (Nat.pair a (Nat.pair y i)))
+    m) n
+| .rfind' f, bound, a =>
+  boundedMinOpt
+    (fun n => Option.isSome (do
+      let v ← evalPrim f bound (Nat.pair a n)
+      guard (v = 0)
+      return v))
+    bound
+
+
+-- Crucial lemma
+lemma evalCorrect (c : Code) (bound n out : ℕ) : evalPrim c bound n = .some out → out ∈ Code.eval c n :=
+by
+  revert bound n out
+  induction c
+  case zero =>
+    intros bound n out h
+    simp [evalPrim] at h
+    cases h
+    simp [Code.eval, pure, PFun.pure]
+  case succ =>
+    intros bound n out h
+    simp [evalPrim] at h
+    cases h
+    simp [Code.eval]
+  case left =>
+    intros bound n out h
+    simp [evalPrim] at h
+    cases h
+    simp [Code.eval]
+  case right =>
+    intros bound n out h
+    simp [evalPrim] at h
+    cases h
+    simp [Code.eval]
+  case pair f g f_ih g_ih =>
+    intros bound n out h
+    simp [evalPrim] at h
+    match fh: (evalPrim f bound n) with
+    | .none =>
+      rw [fh] at h
+      simp [Seq.seq] at h
+    | .some x =>
+      match gh: (evalPrim g bound n) with
+      | .none => rw [gh] at h; simp [Seq.seq] at h
+      | .some y =>
+        rw [fh, gh] at h; simp [Seq.seq] at h
+        simp [Code.eval, Seq.seq]
+        exists x; constructor; apply f_ih; assumption
+        exists y; constructor; apply g_ih <;> assumption
+        assumption
+  case comp f g f_ih g_ih =>
+    intros bound n out h
+    simp [evalPrim] at h
+    simp [Code.eval]
+    match gh: (evalPrim g bound n) with
+    | .none =>
+      rw [gh] at h
+      simp at h
+    | .some x =>
+      rw [gh] at h; simp at h
+      match fh: (evalPrim f bound x) with
+      | .none => rw [fh] at h; simp [Seq.seq] at h
+      | .some y =>
+        rw [fh] at h; simp [Seq.seq] at h; rw [← h]
+        exists x; constructor; apply g_ih; assumption
+        apply f_ih; assumption
+  case prec f g f_ih g_ih =>
+    intros bound n out h
+    simp [evalPrim] at h
+    sorry
+  case rfind' f f_ih =>
+    intros bound n out h
+    simp [evalPrim] at h
+    simp [Code.eval]
+    sorry
+
+-- And evalPrim is primrec
+lemma evalPrimPrimrec (c : Code) : Primrec₂ <| evalPrim c := sorry
+
+theorem REPred_is_Primrec {α : Type} [Primcodable α] (A : Set α) (nonEmpty : A.Nonempty) :
+  REPred A → PrimRecImage A
+:=
+by
+  . sorry
+
+#print Nat.Primrec
+
+theorem Primrec_is_RE {α : Type} [Primcodable α] (f : ℕ → ℕ) (primrec_f : Nat.Primrec f) :
+  ∃ f', Nat.Partrec f' ∧ ∀ n, (f' n).Dom ∧ (f n) ∈ f' n :=
+by
+  cases primrec_f
+  case zero => exact ⟨pure 0,
+    by
+      constructor
+      . apply Nat.Partrec.zero
+      . intros n; simp [pure, PFun.pure]
+  ⟩
+  . sorry
+  . sorry
+  . sorry
+  . sorry
+  . sorry
+  . sorry
+
+theorem Primrec_image_is_REPred {α β : Type} [Primcodable α] [Primcodable β]
+  (B : Set β) (isIPrimrecImage : PrimRecImage B) :
+  REPred B :=
+by
+  simp [REPred]
+  have ⟨f, ⟨prf, h⟩⟩ := isIPrimrecImage
+  sorry
